[michocoq] Stratify opcodes and instructions.
We call opcodes the instructions that do not take subprograms as
argument nor have special treatment in the type-checker or
evaluator. Most of the instructions in Michelson fall into this
category, putting them aside makes the number of constructors of the
instruction ASTs much smaller which is needed when reasoning on the
syntax.

In particular, many optimisations at the Michelson level require to
reason about several terms in these ASTs by nesting destructs which
was not tractable with more than 80 constructors.

src/michocoq/semantics.v
@@ -149,7 +149,7 @@ Module Semantics(C : ContractContext).
       + inversion H; reflexivity.
     - split; intros; subst.
       + constructor. rewrite <- (IHt (stack t)); reflexivity.
-      + inversion H; subst. 
+      + inversion H; subst.
         assert (stack t = S) by (rewrite (IHt S); assumption); subst; reflexivity.
   Qed.
 
@@ -547,6 +547,112 @@ Module Semantics(C : ContractContext).
   amount of gas that is actually required to run the contract because
   in the SEQ case, both instructions are run with gas n *)
 
+  Definition eval_opcode param_ty (env : @proto_env param_ty) {A B : stack_type}
+             (o : @opcode param_ty A B) (SA : stack A) : M (stack B) :=
+    match o, SA with
+      | @APPLY _ a b c D i, (x, (existT _ _ f, SA)) =>
+        Return (existT
+                    _ _
+                    (PUSH _ (data_to_concrete_data _ i x) ;; PAIR ;; f), SA)
+      | DUP, (x, SA) => Return (x, (x, SA))
+      | SWAP, (x, (y, SA)) => Return (y, (x, SA))
+      | UNIT, SA => Return (tt, SA)
+      | EQ, (x, SA) => Return ((x =? 0)%Z, SA)
+      | NEQ, (x, SA) => Return (negb (x =? 0)%Z, SA)
+      | LT, (x, SA) => Return ((x <? 0)%Z, SA)
+      | GT, (x, SA) => Return ((x >? 0)%Z, SA)
+      | LE, (x, SA) => Return ((x <=? 0)%Z, SA)
+      | GE, (x, SA) => Return ((x >=? 0)%Z, SA)
+      | @OR _ _ s, (x, (y, SA)) =>
+        Return (or_fun _ (bitwise_variant_field _ s) x y, SA)
+      | @AND _ _ s, (x, (y, SA)) =>
+        Return (and _ (bitwise_variant_field _ s) x y, SA)
+      | @XOR _ _ s, (x, (y, SA)) =>
+        Return (xor _ (bitwise_variant_field _ s) x y, SA)
+      | @NOT _ _ s, (x, SA) => Return (not _ _ (not_variant_field _ s) x, SA)
+      | @NEG _ _ s, (x, SA) => Return (neg _ (neg_variant_field _ s) x, SA)
+      | ABS, (x, SA) => Return (Z.abs_N x, SA)
+      | ISNAT, (x, SA) =>
+        Return (if (x >=? 0)%Z then (Some (Z.to_N x), SA) else (None, SA))
+      | INT, (x, SA) => Return (Z.of_N x, SA)
+      | @ADD _ _ _ s, (x, (y, SA)) =>
+        let! r := add _ _ _ (add_variant_field _ _ s) x y in
+        Return (r, SA)
+      | @SUB _ _ _ s, (x, (y, SA)) =>
+        let! r := sub _ _ _ (sub_variant_field _ _ s) x y in
+        Return (r, SA)
+      | @MUL _ _ _ s, (x, (y, SA)) =>
+        let! r := mul _ _ _ (mul_variant_field _ _ s) x y in
+        Return (r, SA)
+      | @EDIV _ _ _ s, (x, (y, SA)) =>
+        Return (ediv _ _ _ _ (ediv_variant_field _ _ s) x y, SA)
+      | LSL, (x, (y, SA)) => Return (N.shiftl x y, SA)
+      | LSR, (x, (y, SA)) => Return (N.shiftr x y, SA)
+      | COMPARE, (x, (y, SA)) =>
+        Return (comparison_to_int
+                    (compare _
+                             (data_to_comparable_data _ x)
+                             (data_to_comparable_data _ y)), SA)
+      | @CONCAT _ _ s _, (x, (y, SA)) =>
+        Return (concat _ (stringlike_variant_field _ s) x y, SA)
+      | @CONCAT_list _ _ s _, (l, SA) =>
+        Return (concat_list _ (stringlike_variant_field _ s) l, SA)
+      | @SLICE _ _ i, (n1, (n2, (s, SA))) =>
+        Return (slice _ (stringlike_variant_field _ i) n1 n2 s, SA)
+      | PAIR, (x, (y, SA)) => Return ((x, y), SA)
+      | CAR, ((x, y), SA) => Return (x, SA)
+      | CDR, ((x, y), SA) => Return (y, SA)
+      | EMPTY_SET a, SA => Return (set.empty _ (compare a), SA)
+      | @MEM _ _ _ s _, (x, (y, SA)) =>
+        Return (mem _ _
+                      (mem_variant_field _ _ s)
+                      (data_to_comparable_data _ x)
+                      y, SA)
+      | @UPDATE _ _ _ _ s _, (x, (y, (z, SA))) =>
+        Return (update _ _ _ (update_variant_field _ _ _ s) (data_to_comparable_data _ x) y z, SA)
+      | @SIZE _ _ s, (x, SA) =>
+        Return (N.of_nat (size _ (size_variant_field _ s) x), SA)
+      | EMPTY_MAP k val, SA =>
+        Return (map.empty (comparable_data k) (data val) _, SA)
+      | EMPTY_BIG_MAP k val, SA =>
+        Return (map.empty (comparable_data k) (data val) _, SA)
+      | @GET _ _ _ s _, (x, (y, SA)) =>
+        Return (get _ _ _
+                      (get_variant_field _ _ s)
+                      (data_to_comparable_data _ x)
+                      y, SA)
+      | SOME, (x, SA) => Return (Some x, SA)
+      | NONE _, SA => Return (None, SA)
+      | LEFT _, (x, SA) => Return (inl x, SA)
+      | RIGHT _, (x, SA) => Return (inr x, SA)
+      | CONS, (x, (y, SA)) => Return (cons x y, SA)
+      | NIL _, SA => Return (nil, SA)
+      | TRANSFER_TOKENS, (a, (b, (c, SA))) =>
+        Return (transfer_tokens env _ a b c, SA)
+      | SET_DELEGATE, (x, SA) => Return (set_delegate env x, SA)
+      | BALANCE, SA => Return (balance env, SA)
+      | ADDRESS, (x, SA) => Return (address_ env _ x, SA)
+      | CONTRACT ao p, (x, SA) => Return (contract_ env ao p x, SA)
+      | SOURCE, SA => Return (source env, SA)
+      | SENDER, SA => Return (sender env, SA)
+      | AMOUNT, SA => Return (amount env, SA)
+      | IMPLICIT_ACCOUNT, (x, SA) => Return (implicit_account env x, SA)
+      | NOW, SA => Return (now env, SA)
+      | PACK, (x, SA) => Return (pack env _ x, SA)
+      | UNPACK ty, (x, SA) => Return (unpack env ty x, SA)
+      | HASH_KEY, (x, SA) => Return (hash_key env x, SA)
+      | BLAKE2B, (x, SA) => Return (blake2b env x, SA)
+      | SHA256, (x, SA) => Return (sha256 env x, SA)
+      | SHA512, (x, SA) => Return (sha512 env x, SA)
+      | CHECK_SIGNATURE, (x, (y, (z, SA))) =>
+        Return (check_signature env x y z, SA)
+      | DIG n Hlen, SA => Return (stack_dig SA)
+      | DUG n Hlen, SA => Return (stack_dug SA)
+      | DROP n Hlen, SA =>
+        let (S1, S2) := stack_split SA in Return S2
+      | CHAIN_ID, SA => Return (chain_id_ env, SA)
+    end.
+
   Fixpoint eval {param_ty : self_info} {tff0} (env : @proto_env param_ty) {A : stack_type} {B : stack_type}
            (i : instruction param_ty tff0 A B) (fuel : Datatypes.nat) (SA : stack A) {struct fuel} : M (stack B) :=
     match fuel with
@@ -574,71 +680,11 @@ Module Semantics(C : ContractContext).
         | inl x => eval env (body;; LOOP_LEFT body) n (x, SA)
         | inr y => Return (y, SA)
         end
+      | PUSH a x, SA, _ => Return (concrete_data_to_data _ x, SA)
+      | LAMBDA a b code, SA, _ => Return (existT _ _ code, SA)
       | EXEC, (x, (existT _ tff f, SA)), env =>
         let! (y, tt) := eval (no_self env) f n (x, tt) in
         Return (y, SA)
-      | @APPLY _ a b c D i, (x, (existT _ _ f, SA)), env =>
-        Return (existT
-                    _ _
-                    (PUSH _ (data_to_concrete_data _ i x) ;; PAIR ;; f), SA)
-      | DUP, (x, SA), _ => Return (x, (x, SA))
-      | SWAP, (x, (y, SA)), _ => Return (y, (x, SA))
-      | PUSH a x, SA, _ => Return (concrete_data_to_data _ x, SA)
-      | UNIT, SA, _ => Return (tt, SA)
-      | LAMBDA a b code, SA, _ => Return (existT _ _ code, SA)
-      | EQ, (x, SA), _ => Return ((x =? 0)%Z, SA)
-      | NEQ, (x, SA), _ => Return (negb (x =? 0)%Z, SA)
-      | LT, (x, SA), _ => Return ((x <? 0)%Z, SA)
-      | GT, (x, SA), _ => Return ((x >? 0)%Z, SA)
-      | LE, (x, SA), _ => Return ((x <=? 0)%Z, SA)
-      | GE, (x, SA), _ => Return ((x >=? 0)%Z, SA)
-      | @OR _ _ s, (x, (y, SA)), _ =>
-        Return (or_fun _ (bitwise_variant_field _ s) x y, SA)
-      | @AND _ _ s, (x, (y, SA)), _ =>
-        Return (and _ (bitwise_variant_field _ s) x y, SA)
-      | @XOR _ _ s, (x, (y, SA)), _ =>
-        Return (xor _ (bitwise_variant_field _ s) x y, SA)
-      | @NOT _ _ s, (x, SA), _ => Return (not _ _ (not_variant_field _ s) x, SA)
-      | @NEG _ _ s, (x, SA), _ => Return (neg _ (neg_variant_field _ s) x, SA)
-      | ABS, (x, SA), _ => Return (Z.abs_N x, SA)
-      | ISNAT, (x, SA), _ =>
-        Return (if (x >=? 0)%Z then (Some (Z.to_N x), SA) else (None, SA))
-      | INT, (x, SA), _ => Return (Z.of_N x, SA)
-      | @ADD _ _ _ s, (x, (y, SA)), _ =>
-        let! r := add _ _ _ (add_variant_field _ _ s) x y in
-        Return (r, SA)
-      | @SUB _ _ _ s, (x, (y, SA)), _ =>
-        let! r := sub _ _ _ (sub_variant_field _ _ s) x y in
-        Return (r, SA)
-      | @MUL _ _ _ s, (x, (y, SA)), _ =>
-        let! r := mul _ _ _ (mul_variant_field _ _ s) x y in
-        Return (r, SA)
-      | @EDIV _ _ _ s, (x, (y, SA)), _ =>
-        Return (ediv _ _ _ _ (ediv_variant_field _ _ s) x y, SA)
-      | LSL, (x, (y, SA)), _ => Return (N.shiftl x y, SA)
-      | LSR, (x, (y, SA)), _ => Return (N.shiftr x y, SA)
-      | COMPARE, (x, (y, SA)), _ =>
-        Return (comparison_to_int
-                    (compare _
-                             (data_to_comparable_data _ x)
-                             (data_to_comparable_data _ y)), SA)
-      | @CONCAT _ _ s _, (x, (y, SA)), _ =>
-        Return (concat _ (stringlike_variant_field _ s) x y, SA)
-      | @CONCAT_list _ _ s _, (l, SA), _ =>
-        Return (concat_list _ (stringlike_variant_field _ s) l, SA)
-      | @SLICE _ _ i, (n1, (n2, (s, SA))), _ =>
-        Return (slice _ (stringlike_variant_field _ i) n1 n2 s, SA)
-      | PAIR, (x, (y, SA)), _ => Return ((x, y), SA)
-      | CAR, ((x, y), SA), _ => Return (x, SA)
-      | CDR, ((x, y), SA), _ => Return (y, SA)
-      | EMPTY_SET a, SA, _ => Return (set.empty _ (compare a), SA)
-      | @MEM _ _ _ s _, (x, (y, SA)), _ =>
-        Return (mem _ _
-                      (mem_variant_field _ _ s)
-                      (data_to_comparable_data _ x)
-                      y, SA)
-      | @UPDATE _ _ _ _ s _, (x, (y, (z, SA))), _ =>
-        Return (update _ _ _ (update_variant_field _ _ _ s) (data_to_comparable_data _ x) y z, SA)
       | @ITER _ _ s _ body, (x, SA), env =>
         match iter_destruct _ _ (iter_variant_field _ s) x with
         | None => Return SA
@@ -646,17 +692,6 @@ Module Semantics(C : ContractContext).
           let! SB := eval env body n (a, SA) in
           eval env (ITER body) n (y, SB)
         end
-      | @SIZE _ _ s, (x, SA), _ =>
-        Return (N.of_nat (size _ (size_variant_field _ s) x), SA)
-      | EMPTY_MAP k val, SA, _ =>
-        Return (map.empty (comparable_data k) (data val) _, SA)
-      | EMPTY_BIG_MAP k val, SA, _ =>
-        Return (map.empty (comparable_data k) (data val) _, SA)
-      | @GET _ _ _ s _, (x, (y, SA)), _ =>
-        Return (get _ _ _
-                      (get_variant_field _ _ s)
-                      (data_to_comparable_data _ x)
-                      y, SA)
       | @MAP _ _ _ s _ body, (x, SA), env =>
         let v := (map_variant_field _ _ s) in
         match map_destruct _ _ _ _ v x with
@@ -666,22 +701,16 @@ Module Semantics(C : ContractContext).
           let! (c, SC) := eval env (MAP body) n (y, SB) in
           Return (map_insert _ _ _ _ v a b c, SC)
         end
-      | SOME, (x, SA), _ => Return (Some x, SA)
-      | NONE _, SA, _ => Return (None, SA)
       | IF_NONE bt bf, (b, SA), env =>
         match b with
         | None => eval env bt n SA
         | Some b => eval env bf n (b, SA)
         end
-      | LEFT _, (x, SA), _ => Return (inl x, SA)
-      | RIGHT _, (x, SA), _ => Return (inr x, SA)
       | IF_LEFT bt bf, (b, SA), env =>
         match b with
         | inl a => eval env bt n (a, SA)
         | inr b => eval env bf n (b, SA)
         end
-      | CONS, (x, (y, SA)), _ => Return (cons x y, SA)
-      | NIL _, SA, _ => Return (nil, SA)
       | IF_CONS bt bf, (l, SA), env =>
         match l with
         | cons a b => eval env bt n (a, (b, SA))
@@ -690,35 +719,13 @@ Module Semantics(C : ContractContext).
       | CREATE_CONTRACT g p an f, (a, (b, (c, SA))), env =>
         let (oper, addr) := create_contract env g p an _ a b f c in
         Return (oper, (addr, SA))
-      | TRANSFER_TOKENS, (a, (b, (c, SA))), env =>
-        Return (transfer_tokens env _ a b c, SA)
-      | SET_DELEGATE, (x, SA), env => Return (set_delegate env x, SA)
-      | BALANCE, SA, env => Return (balance env, SA)
-      | ADDRESS, (x, SA), env => Return (address_ env _ x, SA)
-      | CONTRACT ao p, (x, SA), env => Return (contract_ env ao p x, SA)
-      | SOURCE, SA, env => Return (source env, SA)
-      | SENDER, SA, env => Return (sender env, SA)
       | SELF ao H, SA, env => Return (self env ao H, SA)
-      | AMOUNT, SA, env => Return (amount env, SA)
-      | IMPLICIT_ACCOUNT, (x, SA), env => Return (implicit_account env x, SA)
-      | NOW, SA, env => Return (now env, SA)
-      | PACK, (x, SA), env => Return (pack env _ x, SA)
-      | UNPACK ty, (x, SA), env => Return (unpack env ty x, SA)
-      | HASH_KEY, (x, SA), env => Return (hash_key env x, SA)
-      | BLAKE2B, (x, SA), env => Return (blake2b env x, SA)
-      | SHA256, (x, SA), env => Return (sha256 env x, SA)
-      | SHA512, (x, SA), env => Return (sha512 env x, SA)
-      | CHECK_SIGNATURE, (x, (y, (z, SA))), env =>
-        Return (check_signature env x y z, SA)
-      | DIG n Hlen, SA, _ => Return (stack_dig SA)
-      | DUG n Hlen, SA, _ => Return (stack_dug SA)
       | DIP nl Hlen i, SA, env =>
         let (S1, S2) := stack_split SA in
         let! S3 := eval env i n S2 in
         Return (stack_app S1 S3)
-      | DROP n Hlen, SA, _ =>
-        let (S1, S2) := stack_split SA in Return S2
-      | CHAIN_ID, SA, env => Return (chain_id_ env, SA)
+      | Instruction_opcode o, SA, env =>
+        eval_opcode _ env o SA
       end
     end.
 
@@ -754,13 +761,6 @@ Module Semantics(C : ContractContext).
         * destruct st as ([x|y], st).
           -- rewrite IHfuel1; try assumption; reflexivity.
           -- reflexivity.
-        * destruct st as (x, ((tff, f), SA)).
-          f_equal.
-          rewrite IHfuel1.
-          -- reflexivity.
-          -- simpl in Hsucc.
-             apply success_bind_arg in Hsucc.
-             assumption.
         * destruct st as (x, SA).
           generalize Hsucc; clear Hsucc.
           simpl.
@@ -816,6 +816,13 @@ Module Semantics(C : ContractContext).
           -- exact Hsucc.
           -- reflexivity.
           -- exact Hsucc.
+        * destruct st as (x, ((tff, f), SA)).
+          f_equal.
+          rewrite IHfuel1.
+          -- reflexivity.
+          -- simpl in Hsucc.
+             apply success_bind_arg in Hsucc.
+             assumption.
         * simpl in Hsucc.
           destruct (stack_split st); rewrite IHfuel1.
           -- reflexivity.
@@ -838,41 +845,14 @@ Module Semantics(C : ContractContext).
       apply eval_deterministic_le; assumption.
   Qed.
 
-  Definition eval_precond_body
-             (eval_precond_n : forall {self_type},
-                 @proto_env self_type ->
-                 forall {tff0 A B},
-                   instruction self_type tff0 A B ->
-                   (stack B -> Prop) -> stack A -> Prop)
-             {self_type} env tff0 A B
-             (i : instruction self_type tff0 A B)
-             (psi : stack B -> Prop)
-             (SA : stack A) : Prop :=
-    match i, env, psi, SA with
-    | FAILWITH, _, _, _ => false
-    | NOOP, env, psi, st => psi st
-    | SEQ B C, env, psi, st =>
-      eval_precond_n env B (eval_precond_n env C psi) st
-    | IF_ bt bf, env, psi, (b, SA) =>
-      if b then eval_precond_n env bt psi SA
-      else eval_precond_n env bf psi SA
-    | LOOP body, env, psi, (b, SA) =>
-      if b then eval_precond_n env (body;; (LOOP body)) psi SA
-      else psi SA
-    | LOOP_LEFT body, env, psi, (ab, SA) =>
-      match ab with
-      | inl x => eval_precond_n env (body;; LOOP_LEFT body) psi (x, SA)
-      | inr y => psi (y, SA)
-      end
-    | EXEC, env, psi, (x, (existT _ _ f, SA)) =>
-      eval_precond_n (no_self env) f (fun '(y, tt) => psi (y, SA)) (x, tt)
+  Definition eval_precond_opcode {self_type} (env : @proto_env self_type)
+             A B (o : @opcode self_type A B) (psi : stack B -> Prop) (SA : stack A) : Prop :=
+    match o, env, psi, SA with
     | @APPLY _ a b c D i, env, psi, (x, (existT _ _ f, SA)) =>
-      psi (existT _ _ (PUSH _ (data_to_concrete_data _ i x) ;; PAIR ;; f), SA)
+      psi (existT _ _ (PUSH _ (data_to_concrete_data _ i x) ;; Instruction_opcode PAIR ;; f), SA)
     | DUP, env, psi, (x, SA) => psi (x, (x, SA))
     | SWAP, env, psi, (x, (y, SA)) => psi (y, (x, SA))
-    | PUSH a x, env, psi, SA => psi (concrete_data_to_data _ x, SA)
     | UNIT, env, psi, SA => psi (tt, SA)
-    | LAMBDA a b code, env, psi, SA => psi (existT _ _ code, SA)
     | EQ, env, psi, (x, SA) => psi ((x =? 0)%Z, SA)
     | NEQ, env, psi, (x, SA) => psi (negb (x =? 0)%Z, SA)
     | LT, env, psi, (x, SA) => psi ((x <? 0)%Z, SA)
@@ -912,6 +892,73 @@ Module Semantics(C : ContractContext).
       psi (mem _ _ (mem_variant_field _ _ s) (data_to_comparable_data _ x) y, SA)
     | @UPDATE _ _ _ _ s _, env, psi, (x, (y, (z, SA))) =>
       psi (update _ _ _ (update_variant_field _ _ _ s) (data_to_comparable_data _ x) y z, SA)
+    | @SIZE _ _ s, env, psi, (x, SA) => psi (N.of_nat (size _ (size_variant_field _ s) x), SA)
+    | EMPTY_MAP k val, env, psi, SA => psi (map.empty (comparable_data k) (data val) _, SA)
+    | EMPTY_BIG_MAP k val, env, psi, SA => psi (map.empty (comparable_data k) (data val) _, SA)
+    | @GET _ _ _ s _, env, psi, (x, (y, SA)) => psi (get _ _ _ (get_variant_field _ _ s) (data_to_comparable_data _ x) y, SA)
+    | SOME, env, psi, (x, SA) => psi (Some x, SA)
+    | NONE _, env, psi, SA => psi (None, SA)
+    | LEFT _, env, psi, (x, SA) => psi (inl x, SA)
+    | RIGHT _, env, psi, (x, SA) => psi (inr x, SA)
+    | CONS, env, psi, (x, (y, SA)) => psi (cons x y, SA)
+    | NIL _, env, psi, SA => psi (nil, SA)
+    | TRANSFER_TOKENS, env, psi, (a, (b, (c, SA))) =>
+      psi (transfer_tokens env _ a b c, SA)
+    | SET_DELEGATE, env, psi, (x, SA) =>
+      psi (set_delegate env x, SA)
+    | BALANCE, env, psi, SA => psi (balance env, SA)
+    | ADDRESS, env, psi, (x, SA) => psi (address_ env _ x, SA)
+    | CONTRACT ao p, env, psi, (x, SA) => psi (contract_ env ao p x, SA)
+    | SOURCE, env, psi, SA => psi (source env, SA)
+    | SENDER, env, psi, SA => psi (sender env, SA)
+    | AMOUNT, env, psi, SA => psi (amount env, SA)
+    | IMPLICIT_ACCOUNT, env, psi, (x, SA) => psi (implicit_account env x, SA)
+    | NOW, env, psi, SA => psi (now env, SA)
+    | PACK, env, psi, (x, SA) => psi (pack env _ x, SA)
+    | UNPACK ty, env, psi, (x, SA) => psi (unpack env ty x, SA)
+    | HASH_KEY, env, psi, (x, SA) => psi (hash_key env x, SA)
+    | BLAKE2B, env, psi, (x, SA) => psi (blake2b env x, SA)
+    | SHA256, env, psi, (x, SA) => psi (sha256 env x, SA)
+    | SHA512, env, psi, (x, SA) => psi (sha512 env x, SA)
+    | CHECK_SIGNATURE, env, psi, (x, (y, (z, SA))) =>
+      psi (check_signature env x y z, SA)
+    | DIG n Hlen, env, psi, st => psi (stack_dig st)
+    | DUG n Hlen, env, psi, st => psi (stack_dug st)
+    | DROP n Hlen, env, psi, SA =>
+      let (S1, S2) := stack_split SA in psi S2
+    | CHAIN_ID, env, psi, SA => psi (chain_id_ env, SA)
+    end.
+
+  Definition eval_precond_body
+             (eval_precond_n : forall {self_type},
+                 @proto_env self_type ->
+                 forall {tff0 A B},
+                   instruction self_type tff0 A B ->
+                   (stack B -> Prop) -> stack A -> Prop)
+             {self_type} env tff0 A B
+             (i : instruction self_type tff0 A B)
+             (psi : stack B -> Prop)
+             (SA : stack A) : Prop :=
+    match i, env, psi, SA with
+    | FAILWITH, _, _, _ => false
+    | NOOP, env, psi, st => psi st
+    | SEQ B C, env, psi, st =>
+      eval_precond_n env B (eval_precond_n env C psi) st
+    | IF_ bt bf, env, psi, (b, SA) =>
+      if b then eval_precond_n env bt psi SA
+      else eval_precond_n env bf psi SA
+    | LOOP body, env, psi, (b, SA) =>
+      if b then eval_precond_n env (body;; (LOOP body)) psi SA
+      else psi SA
+    | LOOP_LEFT body, env, psi, (ab, SA) =>
+      match ab with
+      | inl x => eval_precond_n env (body;; LOOP_LEFT body) psi (x, SA)
+      | inr y => psi (y, SA)
+      end
+    | EXEC, env, psi, (x, (existT _ _ f, SA)) =>
+      eval_precond_n (no_self env) f (fun '(y, tt) => psi (y, SA)) (x, tt)
+    | PUSH a x, env, psi, SA => psi (concrete_data_to_data _ x, SA)
+    | LAMBDA a b code, env, psi, SA => psi (existT _ _ code, SA)
     | @ITER _ _ s _ body, env, psi, (x, SA) =>
       match iter_destruct _ _ (iter_variant_field _ s) x with
       | None => psi SA
@@ -921,10 +968,6 @@ Module Semantics(C : ContractContext).
           (fun SB => eval_precond_n env (ITER body) psi (y, SB))
           (a, SA)
       end
-    | @SIZE _ _ s, env, psi, (x, SA) => psi (N.of_nat (size _ (size_variant_field _ s) x), SA)
-    | EMPTY_MAP k val, env, psi, SA => psi (map.empty (comparable_data k) (data val) _, SA)
-    | EMPTY_BIG_MAP k val, env, psi, SA => psi (map.empty (comparable_data k) (data val) _, SA)
-    | @GET _ _ _ s _, env, psi, (x, (y, SA)) => psi (get _ _ _ (get_variant_field _ _ s) (data_to_comparable_data _ x) y, SA)
     | @MAP _ _ _ s _ body, env, psi, (x, SA) =>
       let v := (map_variant_field _ _ s) in
       match map_destruct _ _ _ _ v x with
@@ -939,22 +982,16 @@ Module Semantics(C : ContractContext).
                (y, SB))
           (a, SA)
       end
-    | SOME, env, psi, (x, SA) => psi (Some x, SA)
-    | NONE _, env, psi, SA => psi (None, SA)
     | IF_NONE bt bf, env, psi, (b, SA) =>
       match b with
       | None => eval_precond_n env bt psi SA
       | Some b => eval_precond_n env bf psi (b, SA)
       end
-    | LEFT _, env, psi, (x, SA) => psi (inl x, SA)
-    | RIGHT _, env, psi, (x, SA) => psi (inr x, SA)
     | IF_LEFT bt bf, env, psi, (b, SA) =>
       match b with
       | inl a => eval_precond_n env bt psi (a, SA)
       | inr b => eval_precond_n env bf psi (b, SA)
       end
-    | CONS, env, psi, (x, (y, SA)) => psi (cons x y, SA)
-    | NIL _, env, psi, SA => psi (nil, SA)
     | IF_CONS bt bf, env, psi, (l, SA) =>
       match l with
       | cons a b => eval_precond_n env bt psi (a, (b, SA))
@@ -963,35 +1000,12 @@ Module Semantics(C : ContractContext).
     | CREATE_CONTRACT g p an f, env, psi, (a, (b, (c, SA))) =>
       let (oper, addr) := create_contract env g p an _ a b f c in
       psi (oper, (addr, SA))
-    | TRANSFER_TOKENS, env, psi, (a, (b, (c, SA))) =>
-      psi (transfer_tokens env _ a b c, SA)
-    | SET_DELEGATE, env, psi, (x, SA) =>
-      psi (set_delegate env x, SA)
-    | BALANCE, env, psi, SA => psi (balance env, SA)
-    | ADDRESS, env, psi, (x, SA) => psi (address_ env _ x, SA)
-    | CONTRACT ao p, env, psi, (x, SA) => psi (contract_ env ao p x, SA)
-    | SOURCE, env, psi, SA => psi (source env, SA)
-    | SENDER, env, psi, SA => psi (sender env, SA)
     | SELF ao H, env, psi, SA => psi (self env ao H, SA)
-    | AMOUNT, env, psi, SA => psi (amount env, SA)
-    | IMPLICIT_ACCOUNT, env, psi, (x, SA) => psi (implicit_account env x, SA)
-    | NOW, env, psi, SA => psi (now env, SA)
-    | PACK, env, psi, (x, SA) => psi (pack env _ x, SA)
-    | UNPACK ty, env, psi, (x, SA) => psi (unpack env ty x, SA)
-    | HASH_KEY, env, psi, (x, SA) => psi (hash_key env x, SA)
-    | BLAKE2B, env, psi, (x, SA) => psi (blake2b env x, SA)
-    | SHA256, env, psi, (x, SA) => psi (sha256 env x, SA)
-    | SHA512, env, psi, (x, SA) => psi (sha512 env x, SA)
-    | CHECK_SIGNATURE, env, psi, (x, (y, (z, SA))) =>
-      psi (check_signature env x y z, SA)
-    | DIG n Hlen, env, psi, st => psi (stack_dig st)
-    | DUG n Hlen, env, psi, st => psi (stack_dug st)
     | DIP n Hlen i, env, psi, SA =>
       let (S1, S2) := stack_split SA in
       eval_precond_n env i (fun SB => psi (stack_app S1 SB)) S2
-    | DROP n Hlen, env, psi, SA =>
-      let (S1, S2) := stack_split SA in psi S2
-    | CHAIN_ID, env, psi, SA => psi (chain_id_ env, SA)
+    | Instruction_opcode o, env, psi, SA =>
+      eval_precond_opcode env _ _ o psi SA
     end.
 
   Fixpoint eval_precond (fuel : Datatypes.nat) :
@@ -1003,6 +1017,20 @@ Module Semantics(C : ContractContext).
     | S n =>
       @eval_precond_body (@eval_precond n)
     end.
+
+  Lemma eval_precond_opcode_correct {sty env A B} (o : opcode A B) st psi :
+    precond (eval_opcode sty env o st) psi <-> eval_precond_opcode env _ _ o psi st.
+  Proof.
+    destruct o; simpl;
+      try reflexivity;
+      try (destruct st; reflexivity);
+      try (destruct st as (x, (y, st)); reflexivity);
+      try (destruct st as (x, (y, st)); rewrite precond_bind; reflexivity);
+      try (destruct st as (x, (y, (z, SA))); reflexivity);
+      try (destruct st as ((x, y), st); reflexivity).
+    - destruct st as (x, ((tff, y), st)); reflexivity.
+    - destruct (stack_split st); reflexivity.
+  Qed.
 
   Lemma eval_precond_correct {sty env tff0 A B} (i : instruction sty tff0 A B) n st psi :
     precond (eval env i n st) psi <-> eval_precond n env i psi st.
@@ -1024,50 +1052,8 @@ Module Semantics(C : ContractContext).
     - destruct st as ([|], st); simpl.
       + apply (IHn _ _ _ _ _ (i;; LOOP_LEFT i)).
       + reflexivity.
-    - destruct st as (x, ((tff, f), st)).
-      rewrite precond_bind.
-      rewrite <- (IHn _ _ _ _ _ f (x, tt) (fun '(y, tt) => psi (y, st))).
-      apply precond_eqv.
-      intros (y, []).
-      simpl.
-      reflexivity.
-    - destruct st as (x, ((tff, y), st)); reflexivity.
-    - destruct st; reflexivity.
-    - destruct st as (x, (y, st)); reflexivity.
     - reflexivity.
     - reflexivity.
-    - reflexivity.
-    - destruct st; reflexivity.
-    - destruct st; reflexivity.
-    - destruct st; reflexivity.
-    - destruct st; reflexivity.
-    - destruct st; reflexivity.
-    - destruct st; reflexivity.
-    - destruct st as (x, (y, st)); reflexivity.
-    - destruct st as (x, (y, st)); reflexivity.
-    - destruct st as (x, (y, st)); reflexivity.
-    - destruct st; reflexivity.
-    - destruct st; reflexivity.
-    - destruct st; reflexivity.
-    - destruct st; reflexivity.
-    - destruct st; reflexivity.
-    - destruct st as (x, (y, st)); rewrite precond_bind; reflexivity.
-    - destruct st as (x, (y, st)); rewrite precond_bind; reflexivity.
-    - destruct st as (x, (y, st)); rewrite precond_bind; reflexivity.
-    - destruct st as (x, (y, st)); reflexivity.
-    - destruct st as (x, (y, st)); reflexivity.
-    - destruct st as (x, (y, st)); reflexivity.
-    - destruct st as (x, (y, st)); reflexivity.
-    - destruct st as (x, (y, st)); reflexivity.
-    - destruct st; reflexivity.
-    - destruct st; reflexivity.
-    - destruct st as (x, (y, (z, st))); reflexivity.
-    - destruct st as (x, (y, st)); reflexivity.
-    - destruct st as ((x, y), st); reflexivity.
-    - destruct st as ((x, y), st); reflexivity.
-    - reflexivity.
-    - destruct st as (x, (y, st)); reflexivity.
-    - destruct st as (x, (y, (z, st))); reflexivity.
     - destruct st as (x, st).
       destruct (iter_destruct (iter_elt_type collection i) collection
                               (iter_variant_field collection i) x) as [(hd, tl)|].
@@ -1077,9 +1063,6 @@ Module Semantics(C : ContractContext).
         intro SA.
         apply IHn.
       + reflexivity.
-    - reflexivity.
-    - reflexivity.
-    - destruct st as (x, (y, st)); reflexivity.
     - destruct st as (x, st).
       destruct (map_destruct (map_in_type collection b i) b collection
                              (map_out_collection_type collection b i)
@@ -1094,56 +1077,24 @@ Module Semantics(C : ContractContext).
         intros (c, B).
         reflexivity.
       + reflexivity.
-    - destruct st; reflexivity.
-    - reflexivity.
     - destruct st as ([|], st); apply IHn.
-    - destruct st; reflexivity.
-    - destruct st; reflexivity.
     - destruct st as ([|], st); apply IHn.
-    - destruct st as (x, (y, st)); reflexivity.
-    - reflexivity.
     - destruct st as ([|], st); apply IHn.
     - destruct st as (a, (b, (c, SA))).
       destruct (create_contract env g p an _ a b i c).
       reflexivity.
-    - destruct st as (a, (b, (c, SA))).
-      reflexivity.
-    - destruct st as (a, SA).
-      reflexivity.
     - reflexivity.
-    - destruct st as (a, SA).
+    - destruct st as (x, ((tff, f), st)).
+      rewrite precond_bind.
+      rewrite <- (IHn _ _ _ _ _ f (x, tt) (fun '(y, tt) => psi (y, st))).
+      apply precond_eqv.
+      intros (y, []).
+      simpl.
       reflexivity.
-    - destruct st as (a, SA).
-      reflexivity.
-    - reflexivity.
-    - reflexivity.
-    - reflexivity.
-    - reflexivity.
-    - destruct st as (a, SA).
-      reflexivity.
-    - reflexivity.
-    - destruct st as (x, SA).
-      reflexivity.
-    - destruct st as (x, SA).
-      reflexivity.
-    - destruct st as (x, SA).
-      reflexivity.
-    - destruct st as (x, SA).
-      reflexivity.
-    - destruct st as (x, SA).
-      reflexivity.
-    - destruct st as (x, SA).
-      reflexivity.
-    - destruct st as (a, (b, (c, SA))).
-      reflexivity.
-    - reflexivity.
-    - reflexivity.
     - destruct (stack_split st).
       rewrite precond_bind.
       apply IHn.
-    - destruct (stack_split st).
-      reflexivity.
-    - reflexivity.
+    - apply eval_precond_opcode_correct.
   Qed.
 
 End Semantics.
